detype_dom_wf proof

PDDL_Normalization.thy
@@ -199,7 +199,9 @@ begin
   lemma ents_detyped: "\<forall>(n, T) \<in> set (detype_ents ents). T = \<omega>"
     unfolding detype_ents_def
     by (simp add: case_prod_beta' detype_dom_def)
-  
+
+
+
   lemma ac_params_detyped:
     "\<forall>ac \<in> set (actions detype_dom). \<forall>(n, T) \<in> set (parameters ac). T = \<omega>"
     using detype_dom_def detype_ac_def ents_detyped by fastforce
@@ -326,15 +328,15 @@ lemma (in ast_problem) simple_obj_of_type_iff:
 lemma dist_pred: "distinct names \<longleftrightarrow> distinct (map Pred names)"
   by (meson distinct_map inj_onI predicate.inject)
 
-context wf_ast_domain
+context ast_domain
 begin
-  lemmas wf_dom_def = wf_domain[unfolded wf_domain_def]
+  lemmas (in wf_ast_domain) wf_dom_def = wf_domain[unfolded wf_domain_def]
 
-  lemma (in ast_domain) dt_pred_name: "pred (detype_pred pd) = pred pd" by simp
-  lemma (in ast_domain) dt_preds_names:
+  lemma dt_pred_name: "pred (detype_pred pd) = pred pd" by simp
+  lemma dt_preds_names:
     "map pred (detype_preds ps) = map pred ps"
     using dt_pred_name detype_preds_def by simp
-  lemma (in ast_domain) tps_dis:
+  lemma tps_dis:
     "distinct (map pred type_preds)" (is "distinct ?tp_ids")
   proof -
     let ?pred_ids = "map pred (predicates D)"
@@ -349,7 +351,7 @@ begin
   qed
 
   (* TODO simplify *)
-  lemma (in ast_domain) tps_dt_preds_disj:
+  lemma tps_dt_preds_disj:
     "pred ` set type_preds \<inter> pred ` set (detype_preds (predicates D)) = {}"
   proof -
     let ?preds = "map pred (predicates D)"
@@ -378,7 +380,7 @@ begin
     thus ?thesis by simp
   qed
 
-  lemma t_preds_dis:
+  lemma (in wf_ast_domain) t_preds_dis:
     shows "distinct (map pred (predicates detype_dom))"
   proof -
     (* Predicate names are unique because the original predicate names are unchanged
@@ -394,7 +396,7 @@ begin
     thus ?thesis using ast_domain.sel(2) detype_dom_def by presburger
   qed
 
-  lemma (in ast_domain) t_preds_wf:
+  lemma t_preds_wf:
       "\<forall>p \<in> set (predicates detype_dom). ast_domain.wf_predicate_decl detype_dom p"
     proof -
       have "\<forall>p \<in> set (predicates detype_dom). \<forall>T \<in> set (argTs p). T = \<omega>"
@@ -404,16 +406,16 @@ begin
       thus ?thesis by (metis ast_domain.wf_predicate_decl.simps predicate_decl.collapse)
     qed
   
-  lemma (in ast_domain) t_ents_names:
+  lemma t_ents_names:
     "map fst (detype_ents ents) = map fst ents"
     unfolding detype_ents_def by auto
 
-  lemma (in ast_domain) t_ents_dis:
+  lemma t_ents_dis:
     assumes "distinct (map fst ents)"
     shows "distinct (map fst (detype_ents ents))"
     using assms by (metis t_ents_names)
 
-  lemma (in ast_domain) t_ents_wf:
+  lemma t_ents_wf:
     shows "(\<forall>(n,T)\<in>set (detype_ents ents). ast_domain.wf_type detype_dom T)"
     using ents_detyped wf_object by fast
 
@@ -439,7 +441,7 @@ begin
     thus ?thesis using 1 by presburger
   qed
 
-  lemma sig_some:
+  lemma (in wf_ast_domain) sig_some:
     "sig p = Some Ts \<longleftrightarrow> PredDecl p Ts \<in> set (predicates D)"
   proof -
     have "distinct (map pred (predicates D))" using wf_dom_def by simp
@@ -469,7 +471,7 @@ begin
   qed
 
   (* d2.sig maps interchangable *)
-  lemma t_sig_split_b:
+  lemma (in wf_ast_domain) t_sig_split_b:
     "ast_domain.sig detype_dom =
       map_of (map split_pred type_preds) ++ map_of (map split_pred (detype_preds (predicates D)))"
   proof -
@@ -493,7 +495,7 @@ begin
     thus ?thesis using t_sig_split_a by simp
   qed
 
-  lemma t_sig_some:
+  lemma (in wf_ast_domain) t_sig_some:
     "ast_domain.sig detype_dom p \<noteq> None \<longleftrightarrow>
       (p \<in> pred ` set (predicates D))
       \<or> (p \<in> pred_for_type ` set type_names)"
@@ -526,7 +528,7 @@ begin
 
   (* Using distinctness of predicates is a shortcut here.
      It's technically not required because the order of predicates is unchanged.*)
-  lemma t_preds_arity:
+  lemma (in wf_ast_domain) t_preds_arity:
     assumes "sig p = Some Ts"
     shows "ast_domain.sig detype_dom p = Some (replicate (length Ts) \<omega>)"
   proof -
@@ -545,6 +547,7 @@ begin
     by (simp add: map_of_eq_None_iff)
 
   (* formulas *)
+
   lemma "constT x \<noteq> None \<longleftrightarrow> (x \<in> fst ` set (consts D))"
     using constT_def by (simp add: map_of_eq_None_iff)
 
@@ -555,13 +558,64 @@ begin
     have "map fst ents = map fst (detype_ents ents)" using t_ents_names by metis
     hence x: "x \<in> fst ` set (detype_ents ents)" using assms by (metis image_set)
     have "\<forall>T \<in> snd ` set (detype_ents ents). T = \<omega>"
-      using detype_dom_def ents_detyped by fastforce
+      using ents_detyped by fastforce
     thus ?thesis
       using x img_snd map_of_SomeD map_of_eq_None_iff option.exhaust by metis
   qed
 
-  lemma t_constT: "x \<in> fst ` set (consts D) \<Longrightarrow> ast_domain.constT detype_dom x = Some \<omega>"
-    using detype_dom_def ast_domain.constT_def t_entT by simp
+  lemma "\<forall>y \<in> snd ` set m. y = r \<Longrightarrow> x \<in> fst ` set m \<Longrightarrow> map_of m x = Some r"
+    by (metis img_snd in_fst_imageE map_of_SomeD weak_map_of_SomeI)
+
+  lemma "snd ` set m = {r} \<Longrightarrow> x \<in> fst ` set m \<Longrightarrow> map_of m x = Some r"
+    by (metis emptyE img_snd in_fst_imageE insertE map_of_SomeD weak_map_of_SomeI)
+
+  lemma t_entT_alt:
+    shows "map_of ents x \<noteq> None \<longleftrightarrow> map_of (detype_ents ents) x = Some \<omega>"
+  proof -
+    have 1: "\<forall>T \<in> snd ` set (detype_ents ents). T = \<omega>" using ents_detyped by fastforce
+    have "map_of ents x \<noteq> None \<longleftrightarrow> x \<in> fst ` set ents" using map_of_eq_None_iff by metis
+    also have "... \<longleftrightarrow> x \<in> fst ` set (detype_ents ents)" using t_ents_names by (metis list.set_map)
+    ultimately show ?thesis using 1
+      by (metis map_of_eq_None_iff option.distinct(1) t_entT)
+  qed
+
+  lemma t_entT_None:
+    shows "map_of ents x = None \<longleftrightarrow> map_of (detype_ents ents) x = None" sorry
+
+  lemma t_constT: "constT c \<noteq> None \<longleftrightarrow> ast_domain.constT detype_dom c = Some \<omega>"
+    using t_entT_alt ast_domain.constT_def detype_dom_def by fastforce
+
+  lemma "m1 x = Some y \<or> m1 x = None \<and> m2 x = Some y \<Longrightarrow> (m2 ++ m1) x = Some y"
+    by (simp add: map_add_Some_iff)
+
+  lemma (in ast_problem) t_objT: "objT c \<noteq> None \<longleftrightarrow> ast_problem.objT detype_prob c = Some \<omega>"
+  proof -
+    interpret p2 : ast_problem detype_prob .
+    have o1: "objT = map_of (objects P) ++ constT" using objT_def by simp
+
+    have "objT c \<noteq> None \<longleftrightarrow> constT c \<noteq> None \<or> constT c = None \<and> map_of (objects P) c \<noteq> None" using objT_def by auto
+    also have "... \<longleftrightarrow> p2.constT c = Some \<omega> \<or> p2.constT c = None \<and> map_of (objects P) c \<noteq> None"
+      using t_constT t_entT_None detype_prob_def sorry
+    also have "... \<longleftrightarrow> p2.constT c = Some \<omega> \<or> p2.constT c = None \<and> map_of (objects detype_prob) c = Some \<omega>"
+      using t_entT_alt detype_prob_def by fastforce
+    also have "... \<longleftrightarrow> p2.constT c = Some \<omega> \<or> p2.constT c = None \<and> map_of (objects detype_prob) c = Some \<omega>"
+      using t_entT_None detype_prob_def by fastforce
+    also have "... \<longleftrightarrow> (map_of (objects detype_prob) ++ p2.constT) c = Some \<omega>" using map_add_Some_iff sorry
+    (* also have "... \<longleftrightarrow> p2.objT c = Some \<omega>" sorry *)
+
+    ultimately show ?thesis sorry
+  qed
+
+
+  lemma t_cnstT_some:
+    assumes "ty_term vT (map_of cnsts) (term.CONST x) \<noteq> None"
+    shows "ty_term vT' (map_of (detype_ents cnsts)) (term.CONST x) = Some \<omega>"
+    using assms t_entT by (metis map_of_eq_None_iff ty_term.simps(2))
+
+  lemma t_varT_some:
+    assumes "ty_term (map_of vars) cT (term.VAR x) \<noteq> None"
+    shows "ty_term (map_of (detype_ents vars)) cT' (term.VAR x) = Some \<omega>"
+    using assms t_entT by (metis map_of_eq_None_iff ty_term.simps(1))
 
   lemma t_tyt_some:
     assumes "ty_term (map_of vars) (map_of cnsts) e \<noteq> None"
@@ -595,11 +649,10 @@ begin
   qed
 
   thm wf_pred_atom.simps
-  lemma
+  lemma (in wf_ast_domain) t_atom_wf:
     assumes "\<forall>e. tyt e \<noteq> None \<longrightarrow> tyt2 e = Some \<omega>"
       "wf_atom tyt a"
-    shows
-      "ast_domain.wf_atom detype_dom tyt2 a"
+    shows "ast_domain.wf_atom detype_dom tyt2 a"
   proof -
     interpret d2 : ast_domain detype_dom .
     from assms show ?thesis
@@ -619,6 +672,39 @@ begin
     qed simp
   qed
 
+  lemma (in wf_ast_domain) t_fmla_wf:
+    assumes "\<forall>e. tyt e \<noteq> None \<longrightarrow> tyt2 e = Some \<omega>"
+      "wf_fmla tyt \<phi>"
+    shows "ast_domain.wf_fmla detype_dom tyt2 \<phi>"
+    using assms apply (induction \<phi>)
+    using t_atom_wf ast_domain.wf_fmla.simps(1) apply blast
+    using ast_domain.wf_fmla.simps(2) apply blast
+    using ast_domain.wf_fmla.simps(5) apply blast
+    using ast_domain.wf_fmla.simps(3) apply blast
+    using ast_domain.wf_fmla.simps(4) apply blast
+    using ast_domain.wf_fmla.simps(6) by metis
+
+  lemma (in wf_ast_domain) t_fmla_atom_wf:
+    assumes "\<forall>e. tyt e \<noteq> None \<longrightarrow> tyt2 e = Some \<omega>"
+      "wf_fmla_atom tyt \<phi>"
+    shows "ast_domain.wf_fmla_atom detype_dom tyt2 \<phi>"
+    using assms
+    by (simp add: ast_domain.wf_fmla_atom_alt t_fmla_wf)
+
+  lemma wf_effect_alt:
+    "wf_effect tyt \<epsilon> \<longleftrightarrow>
+       (\<forall>ae\<in>set (adds \<epsilon>). wf_fmla_atom tyt ae)
+       \<and> (\<forall>de\<in>set (dels \<epsilon>).  wf_fmla_atom tyt de)"
+    using wf_effect.simps ast_effect.collapse
+    by metis (* TODO how to just manipulate this lemma with options? *)
+
+  lemma (in wf_ast_domain) t_eff_wf:
+    assumes "\<forall>e. tyt e \<noteq> None \<longrightarrow> tyt2 e = Some \<omega>"
+      "wf_effect tyt \<epsilon>"
+    shows "ast_domain.wf_effect detype_dom tyt2 \<epsilon>"
+    using assms ast_domain.wf_effect_alt t_fmla_atom_wf by blast
+
+
   (* actions *)
   abbreviation (in ast_domain) "ac_name \<equiv> ast_action_schema.name"
   (* abbreviation (in ast_domain) "ac_params \<equiv> ast_action_schema.parameters" \<comment> just use \<open>parameters\<close> *)
@@ -629,7 +715,7 @@ begin
     by (simp add: detype_ac_def)
   lemma t_acs_names: "map ac_name (map detype_ac acs) = map ac_name acs"
     by (simp add: t_ac_name)
-  lemma t_acs_dis:
+  lemma (in wf_ast_domain) t_acs_dis:
     "distinct (map ac_name (map detype_ac (actions D)))"
     using t_acs_names wf_dom_def by metis
 
@@ -645,38 +731,137 @@ begin
     using wf_action_schema.simps
     by (metis ast_action_schema.collapse)
 
-  lemma (in ast_domain) t_ac_wf:
-    assumes "wf_action_schema a"
+  lemma t_ac_tyt:
+    assumes "ty_term (map_of (parameters a)) constT x \<noteq> None"
+    shows "ty_term (map_of (parameters (detype_ac a))) (ast_domain.constT detype_dom) x = Some \<omega>"
+    using assms detype_ac_def detype_dom_def t_tyt_some ast_domain.constT_def by auto
+
+  (* fun type_precond :: "(variable \<times> type) \<Rightarrow> term atom formula" where
+    "type_precond (v, T) =
+      disj_fmlas (map (Atom \<circ> (\<lambda>p. predAtm p [term.VAR v])) (type_conds T))"
+  
+  fun param_precond :: "(variable \<times> type) list \<Rightarrow> term atom formula" where
+    "param_precond params = conj_fmlas (map type_precond params)" *)
+
+  lemma conj_fmlas_wf:
+    assumes "\<forall>\<phi> \<in> set \<phi>s. wf_fmla tyt \<phi>"
+    shows "wf_fmla tyt (conj_fmlas \<phi>s)"
+    using assms apply (induction \<phi>s)
+    apply simp_all
+    by (metis ast_domain.wf_fmla.simps(3) conj_fmlas.simps(2-3) neq_Nil_conv)
+
+  lemma disj_fmlas_wf:
+    assumes "\<forall>\<phi> \<in> set \<phi>s. wf_fmla tyt \<phi>"
+    shows "wf_fmla tyt (disj_fmlas \<phi>s)"
+    using assms apply (induction \<phi>s)
+    apply simp_all
+    by (metis ast_domain.wf_fmla.simps(4) disj_fmlas.simps(2-3) neq_NilE)
+
+(* disj_fmlas (map (Atom \<circ> (\<lambda>p. predAtm p [term.VAR v])) (type_conds T)) *)
+
+  lemma "\<forall>ent. snd (detype_ent ent) = \<omega>"
+    by simp
+
+  lemma params_ts_wf:
+    assumes "wf_action_params a" "p \<in> set (parameters a)"
+    shows "wf_type (snd p)"
+    using assms wf_action_params_def by blast
+
+  lemma set_type_names: "set type_names = insert ''object'' (fst ` set (types D))" by auto
+
+  lemma params_ts_exist: (* somehow this isn't trivial for the solver *)
+    assumes "wf_action_params a" "p \<in> set (parameters a)"
+    shows "\<forall>t \<in> set (primitives (snd p)). t \<in> insert ''object'' (set type_names)"
+    using assms params_ts_wf set_type_names
+    by (metis wf_type_iff_listed insertI2 type.exhaust_sel)
+
+  lemma (in wf_ast_domain) type_precond_wf: (* TODO simplify if possible *)
+    assumes "wf_action_params a" "p \<in> set (parameters a)"
+    shows "ast_domain.wf_fmla detype_dom
+      (ty_term (map_of (parameters (detype_ac a))) egal)
+      (type_precond p)"
+  proof -
+    interpret d2 : ast_domain detype_dom .
+    let ?tyt = "ty_term (map_of (parameters a)) egal"
+    let ?tyt2 = "ty_term (map_of (parameters (detype_ac a))) egal"
+
+    have "?tyt (term.VAR (fst p)) \<noteq> None" using assms detype_ac_def
+      by (metis imageI map_of_eq_None_iff ty_term.simps(1))
+    hence 1: "?tyt2 (term.VAR (fst p)) = Some \<omega>" using t_varT_some
+      by (simp add: detype_ac_def)
+
+    have "\<forall>t \<in> set (primitives (snd p)). d2.wf_fmla ?tyt2 (Atom (predAtm (pred_for_type t) [term.VAR (fst p)]))"
+    proof
+      fix t assume t: "t \<in> set (primitives (snd p))"
+      have "t \<in> insert ''object'' (set type_names)" using assms params_ts_exist t by simp
+      hence "PredDecl (pred_for_type t) [\<omega>] \<in> set type_preds" using type_preds_def by fastforce
+      moreover have "set type_preds \<subseteq> set (predicates detype_dom)" using detype_dom_def by simp
+      ultimately have "PredDecl (pred_for_type t) [\<omega>] \<in> set (predicates detype_dom)" by auto
+      hence 2: "d2.sig (pred_for_type t) = Some [\<omega>]" using detype_dom_def
+        by (metis d2.sig_def pred_resolve t_preds_dis) (* not true outside of restr_dom because action params need not wf *)
+      from 1 2 show "d2.wf_fmla ?tyt2 (Atom (predAtm (pred_for_type t) [term.VAR (fst p)]))"
+        using d2.of_type_refl d2.is_of_type_def by fastforce
+    qed
+
+    hence "\<forall>\<phi> \<in> set (map (Atom \<circ> (\<lambda>pn. predAtm pn [term.VAR (fst p)])) (type_conds (snd p))). d2.wf_fmla ?tyt2 \<phi>"
+      by simp
+    hence "d2.wf_fmla ?tyt2 (disj_fmlas (map (Atom \<circ> (\<lambda>pn. predAtm pn [term.VAR (fst p)])) (type_conds (snd p))))"
+      using d2.disj_fmlas_wf by metis
+    thus "d2.wf_fmla ?tyt2 (type_precond p)"
+      by (metis prod.collapse type_precond.simps)
+  qed
+
+  lemma (in wf_ast_domain) t_param_precond_wf:
+    assumes "wf_action_params a"
+    shows "ast_domain.wf_fmla detype_dom
+    (ty_term (map_of (parameters (detype_ac a))) egal)
+    (param_precond (parameters a))"
+  proof -
+    interpret d2 : ast_domain detype_dom .
+    let ?tyt2 = "ty_term (map_of (parameters (detype_ac a))) egal"
+    have "param_precond (parameters a) = conj_fmlas (map type_precond (parameters a))"
+      by simp
+    have "\<forall>p \<in> set (parameters a). d2.wf_fmla
+      ?tyt2
+      (type_precond p)" using type_precond_wf assms by simp
+    hence "\<forall>\<phi> \<in> set (map type_precond (parameters a)). d2.wf_fmla ?tyt2 \<phi>" by simp
+    hence "d2.wf_fmla ?tyt2 (conj_fmlas (map type_precond (parameters a)))"
+      using d2.conj_fmlas_wf by blast
+    thus ?thesis by simp
+  qed
+
+  lemma (in restr_domain) t_ac_wf:
+    assumes "a \<in> set (actions D)"
     shows "ast_domain.wf_action_schema detype_dom (detype_ac a)"
   proof -
     interpret d2 : ast_domain detype_dom .
     let ?a2 = "detype_ac a"
-    define tyt where tyt: "tyt \<equiv> ty_term (map_of (parameters a)) constT"
-    from assms have 1: "distinct (map fst (parameters a))" using wf_ac_expanded by metis
-    from assms tyt have 2: "wf_fmla tyt (ac_pre a)" using wf_ac_expanded by metis
-    from assms tyt have 3: "wf_effect tyt (ac_eff a)" using wf_ac_expanded by metis
-  
-    define tyt2 where tyt2: "tyt2 \<equiv> ty_term (map_of (parameters ?a2)) d2.constT"
-    have ps: "parameters ?a2 = detype_ents (parameters a)" by (simp add: detype_ac_def)
-    hence c1: "distinct (map fst (parameters ?a2))" using 1 t_ents_dis by auto
-    text \<open>This fact is not required for \<open>wf_action_schema\<close> but it should be, maybe\<close>
-    from ps have cx: "(\<forall>(n,T)\<in>set (parameters ?a2). d2.wf_type T)"
-      using t_ents_wf by metis
-  
-    have c2a: "d2.wf_fmla tyt2 (param_precond (parameters a))" sorry
-    have c2b: "d2.wf_fmla tyt2 (ac_pre a)" sorry
-    from c2a c2b have c2: "d2.wf_fmla tyt2 (ac_pre ?a2)" by (simp add: detype_ac_def)
-    have "d2.wf_effect tyt2 (ac_eff a)" sorry
-    hence c3: "d2.wf_effect tyt2 (ac_eff ?a2)" by (simp add: detype_ac_def)
-  
-    from c1 c2 c3 tyt2 show ?thesis using d2.wf_ac_expanded by simp
+    let ?tyt = "ty_term (map_of (parameters a)) constT"
+    let ?tyt2 = "ty_term (map_of (parameters (detype_ac a))) d2.constT"
+    have tyt_om: "\<forall>x. ?tyt x \<noteq> None \<longrightarrow> ?tyt2 x = Some \<omega>" using t_ac_tyt by simp
+
+    from assms have wfa: "wf_action_schema a" using wf_domain wf_domain_def by simp
+    from assms have "distinct (map fst (parameters a))" using wfa wf_ac_expanded by metis
+    hence c1: "distinct (map fst (parameters ?a2))" using t_ents_dis detype_ac_def by auto
+    from assms have "wf_fmla ?tyt (ac_pre a)" using wfa wf_ac_expanded by metis
+    hence c2b: "d2.wf_fmla ?tyt2 (ac_pre a)" using tyt_om t_fmla_wf by blast
+    from assms have "wf_effect ?tyt (ac_eff a)" using wfa wf_ac_expanded by metis
+    hence "d2.wf_effect ?tyt2 (ac_eff a)"
+      using tyt_om ast_domain.wf_effect.simps t_eff_wf detype_ac_def by blast
+    hence c3: "d2.wf_effect ?tyt2 (ac_eff ?a2)" using detype_ac_def by simp
+
+    have "wf_action_params a" using restrD restrict_dom_def assms by simp
+    note c2a = t_param_precond_wf[OF this]
+    from c2a c2b have c2: "d2.wf_fmla ?tyt2 (ac_pre ?a2)" by (simp add: detype_ac_def)
+
+    from c1 c2 c3 show ?thesis using d2.wf_ac_expanded by simp
   qed
 
-  lemma t_acs_wf:
+  lemma (in restr_domain) t_acs_wf:
     shows "(\<forall>a\<in>set (map detype_ac (actions D)). ast_domain.wf_action_schema detype_dom a)"
     using detype_dom_def wf_dom_def t_ac_wf by simp
 
-  theorem detype_dom_wf:
+  theorem (in restr_domain) detype_dom_wf:
     shows "ast_domain.wf_domain detype_dom"
   proof -
     interpret d2 : ast_domain detype_dom .
@@ -699,12 +884,53 @@ begin
   qed
 end
 
+context ast_problem
+begin
+
+lemmas (in wf_ast_problem) wf_prob_def = wf_problem[unfolded wf_problem_def]
+
+thm detype_prob_def
+
+lemma (in wf_ast_problem) t_init_dis: "distinct (init detype_prob)"
+  sorry
+
+thm wf_ast_domain.t_fmla_wf
+
+theorem (in restr_problem) detype_prob_wf:
+  shows "ast_problem.wf_problem detype_prob"
+proof -
+  interpret p2 : ast_problem detype_prob .
+
+  note p2.wf_problem_def
+  note detype_prob_def
+
+  note c1 = detype_dom_wf
+  have "distinct (map fst (objects P) @ map fst (consts D))" using wf_prob_def by simp
+  hence c2: "distinct (map fst (detype_ents (objects P)) @ map fst (detype_ents (consts D)))"
+    using t_ents_names by metis
+  have c3: "\<forall>(n, y)\<in>set (objects detype_prob). p2.wf_type y" using t_ents_wf detype_prob_def by fastforce
+  note c4 = t_init_dis
+  have c5: "p2.wf_world_model (set (init detype_prob))" sorry
+
+  have c6a: "\<forall>e. objT e \<noteq> None \<longrightarrow> p2.objT e = Some \<omega>" sorry
+  have c6b: "wf_fmla objT (goal detype_prob)" using detype_prob_def wf_prob_def by simp
+  have c6: "p2.wf_fmla p2.objT (goal detype_prob)"
+    using t_fmla_wf[OF c6a c6b] detype_prob_def by simp
+  from c1 c2 c3 c4 c5 c6 show ?thesis
+    using p2.wf_problem_def detype_prob_def detype_dom_def by simp
+qed
+end
+
+
 (* ---------------------- Milestones ------------------------- *)
 
 
 (* TODO update locale hierarchy accordingly *)
-lemma (in ast_problem) "ast_problem.wf_problem detype_prob"
-  oops
+lemma (in restr_domain) "ast_domain.wf_domain detype_dom"
+  by (rule detype_dom_wf)
+
+lemma (in restr_problem) "ast_problem.wf_problem detype_prob"
+  by (rule detype_prob_wf)
 
 lemma "ast_domain.wf_domain D \<Longrightarrow> typeless_dom (detype_dom D)"
   oops
