PDDL_Normalization_code.thy
@@ -1,0 +1,114 @@
+theory PDDL_Normalization_code
+  imports "AI_Planning_Languages_Semantics.PDDL_STRIPS_Semantics"
+    Graph_Funs String_Shenanigans
+begin
+text \<open>Check if a formula consists of only (nested) conjunctions of literals.\<close>
+fun only_conj :: "'a formula \<Rightarrow> bool" where
+  "only_conj (Atom a) \<longleftrightarrow> True" |
+  "only_conj \<bottom> \<longleftrightarrow> True" |
+  "only_conj (\<^bold>\<not> (Atom a)) \<longleftrightarrow> True" |
+  "only_conj (\<phi> \<^bold>\<and> \<psi>) \<longleftrightarrow> only_conj \<phi> \<and> only_conj \<psi>" |
+
+  "only_conj (\<^bold>\<not> _) \<longleftrightarrow> False" |
+  "only_conj (_ \<^bold>\<or> _) \<longleftrightarrow> False" |
+  "only_conj (_ \<^bold>\<rightarrow> _) \<longleftrightarrow> False"
+
+subsection \<open> Type Normalization \<close>
+abbreviation "type_names D \<equiv> remdups (''object'' # map fst (types D))"
+
+abbreviation singleton_types :: "('a \<times> type) list \<Rightarrow> bool" where
+  "singleton_types os \<equiv> (\<forall>(_, t) \<in> set os. length (primitives t) = 1)"
+
+definition const_single_types :: "ast_domain \<Rightarrow> bool" where
+  "const_single_types D \<equiv> singleton_types (consts D)"
+
+definition objs_single_types :: "ast_problem \<Rightarrow> bool" where
+  ost_aux: "objs_single_types P \<equiv>
+    const_single_types (domain P)
+    \<and> singleton_types (objects P)"
+
+definition restricted_pddl :: "ast_problem \<Rightarrow> bool" where
+  "restricted_pddl P \<longleftrightarrow> objs_single_types P"
+
+definition pred_names :: "ast_domain \<Rightarrow> name list" where
+  "pred_names D = map (predicate.name \<circ> pred) (predicates D)"
+
+fun pred_for_type :: "ast_domain \<Rightarrow> name \<Rightarrow> predicate" where
+  "pred_for_type D t = Pred (safe_prefix (pred_names D) @ t)"
+
+fun type_preds :: "ast_domain \<Rightarrow> predicate_decl list" where
+  "type_preds D = map ((\<lambda>p. PredDecl p [Either [''object'']]) \<circ> (pred_for_type D)) (type_names D)"
+
+fun supertype_preds :: "ast_domain \<Rightarrow> name \<Rightarrow> predicate list" where
+  "supertype_preds D t = map (pred_for_type D) (reachable_nodes (types D) t)"
+
+text \<open>This only works for singleton types on purpose.\<close>
+fun supertype_facts_for :: "ast_domain \<Rightarrow> (object \<times> type) \<Rightarrow> object atom formula list" where
+  "supertype_facts_for D (n, Either [t]) =
+    map (Atom \<circ> (\<lambda>p. predAtm p [n])) (supertype_preds D t)"
+
+fun type_conds :: "ast_domain \<Rightarrow> type \<Rightarrow> predicate list" where
+  "type_conds D (Either ts) = map (pred_for_type D) ts"
+
+fun disj_fmlas :: "'a formula list \<Rightarrow> 'a formula" where
+  "disj_fmlas [] = Bot" |
+  "disj_fmlas [f] = f" |
+  "disj_fmlas (f # fs) = f \<^bold>\<or> disj_fmlas fs"
+
+fun conj_fmlas :: "'a formula list \<Rightarrow> 'a formula" where
+  "conj_fmlas [] = \<^bold>\<not> \<bottom>" |
+  "conj_fmlas [f] = f" |
+  "conj_fmlas (f # fs) = f \<^bold>\<and> conj_fmlas fs"
+
+fun type_precond :: "ast_domain \<Rightarrow> (variable \<times> type) \<Rightarrow> term atom formula" where
+  "type_precond D (v, T) =
+    disj_fmlas (map (Atom \<circ> (\<lambda>p. predAtm p [term.VAR v])) (type_conds D T))"
+
+fun param_precond :: "ast_domain \<Rightarrow> (variable \<times> type) list \<Rightarrow> term atom formula" where
+  "param_precond D params = conj_fmlas (map (type_precond D) params)"
+
+fun detype_ent :: "('ent \<times> type) \<Rightarrow> ('ent \<times> type)" where
+  "detype_ent (n, T) = (n, Either [''object''])"
+
+definition detype_ents :: "('ent \<times> type) list \<Rightarrow> ('ent \<times> type) list" where
+  "detype_ents params \<equiv> map detype_ent params"
+
+fun detype_ac :: "ast_domain \<Rightarrow> ast_action_schema \<Rightarrow> ast_action_schema" where
+  "detype_ac D (Action_Schema nam params pre eff) =
+    Action_Schema nam (detype_ents params) (param_precond D params \<^bold>\<and> pre) eff"
+
+fun detype_preds :: "predicate_decl list \<Rightarrow> predicate_decl list" where
+  "detype_preds preds =
+    map (\<lambda>pd. PredDecl (pred pd) (replicate (length (argTs pd)) (Either [''object'']))) preds"
+
+fun detype_dom :: "ast_domain \<Rightarrow> ast_domain" where
+  "detype_dom D =
+    Domain
+      []
+      (type_preds D @ detype_preds (predicates D))
+      (detype_ents (consts D))
+      (map (detype_ac D) (actions D))"
+
+fun supertype_facts :: "ast_domain \<Rightarrow> (object \<times> type) list \<Rightarrow> object atom formula list" where
+  "supertype_facts D objs = concat (map (supertype_facts_for D) objs)"
+
+fun detype_prob :: "ast_problem \<Rightarrow> ast_problem" where
+  "detype_prob (Problem d objs i g) =
+    Problem
+      (detype_dom d)
+      (detype_ents objs)
+      (supertype_facts d objs @ supertype_facts d (consts d) @ i)
+      g"
+
+definition typeless_dom :: "ast_domain \<Rightarrow> bool" where
+  "typeless_dom D = undefined"
+
+definition typeless_prob :: "ast_problem \<Rightarrow> bool" where
+  "typeless_prob P = undefined"
+
+subsection \<open>Complete Normalization\<close>
+
+definition normalized_prob :: "ast_problem \<Rightarrow> bool" where
+  "normalized_prob P \<equiv> typeless_prob P \<and> undefined"
+
+end
